semantics/Util.v
@@ -3,6 +3,14 @@ Require Import Coq.Strings.String.
 Require Import SEM.State.
 
 
+Require Import Coq.FSets.FMapFacts.
+Require Import Coq.FSets.FSetFacts.
+
+(* Proof helper for Sets and Maps *)
+Module Import P := WProperties_fun Loc_as_OT MemMap.
+Module Import FMapFact := P.F.
+Module Import FSetFact := WFacts_fun Loc_as_OT LocSet.
+
 
 (* Useful variables *)
 Definition W : string := "W".
